\begin{frame}[fragile]{Functors compose with Functors}
	Let's start from an example
\begin{lstlisting}[language=scala]
val v = List(Option(1), None, Option(3))
val f1: Int => String = _ + "a"
v.applyMap(x => x.applyMap(f1)) //List(Some(1a), None, Some(3a))
\end{lstlisting}
	If we have a functor of a functor we can compose $map$ in a simple (and intuitive) way: $map(v)(x => map(x)(f1))$.
\end{frame}

\begin{frame}[fragile]{Monads don't compose with monads (1)}
	Again, let's start from an example
\begin{lstlisting}[language=scala]
val v = List(Option(1), None, Option(3))
val f2: Int => List[Option[String]] = x => List(Some(x + "a"))
v.applyBind(x => x.applyBind(f2)) // COMPILE ERROR
\end{lstlisting}
	If we have a monads of a monads we \textbf{cannot} compose $bind$ in a simple (and intuitive) way: $bind(v)(x => bind(x)(f2))$.
	We would have type mismatch error. 	
\end{frame}

\begin{frame}[fragile]{Monads don't compose with monads (2)}	
	A solution could be
\begin{lstlisting}[language=scala]
v.applyBind {
	case None => ListMonad.unit(None) // List(None)
	case Some(x) => f2(x)
} //List(Some(1a), None, Some(3a))
\end{lstlisting}	
	This yields boilerplate code (again...).

	Note also that now Option could be or not a monad because we don't use bind or unit of Option. 
	So the problem is related to a monad whose internal type is of the form $C[A]$.
\end{frame}

\begin{frame}[fragile]{Transformer}
	Monad transformers are monads whose internal type is of the form $C[A]$, 
	so they are monad of type $M1[M2[A]]$ with an additional method $lift$.
	\pause 
	They have the same laws of monad, plus:
	\begin{enumerate}[<+->]
        \item Law 1: given an object $obj$ we have that
			$lift(unit(obj)) = unit(obj)$ where the unit call on the left is
          	a monad method and unit on the right is a transformer
          	method.
		\item Law 2: given a function $f$ and a monad $m$ we have that $lift(bind(m)(f)) = bind(lift(m))(lift \circ f)$ where the
			bind call on the left is a monad method and the
			bind on the right is a transformer method.
	\end{enumerate}
\end{frame}

\begin{frame}[fragile]{Transformer - Implementation (1)}
	We'll use type classes to implement monad transformers.
\begin{lstlisting}[language=scala]
trait Transformer[M1[_], M2[_]] {
	implicit def monadM1: Monad[M1]	
	def bind[A, B](fa: M1[M2[A]])(f: A => M1[M2[B]]): M1[M2[B]]
	def unit[A](a: A): M1[M2[A]]
	def lift[A](fa: M1[A]): M1[M2[A]]
	final def join[A](fa: M1[M2[M1[M2[A]]]]): M1[M2[A]] =
		bind(fa)(m => m)
	final def map[A, B](fa: M1[M2[A]])(f: A => B): M1[M2[B]] =
		bind(fa)(a => unit(f(a)))
}
\end{lstlisting}
\end{frame}

\begin{frame}[fragile]{Transformer - Implementation (2)}	
	Let's create an Option transformer, called OptionT.
\begin{lstlisting}[language=scala]
trait OptionT[M1[_]] extends Transformer[M1, Option] {
	override def bind[A, B](fa: M1[Option[A]])(f: A => M1[Option[B]]): M1[Option[B]] = {
		monadM1.bind(fa) {
			case None => monadM1.unit(None)
			case Some(a) => f(a)
		}
	}
	override def lift[A](fa: M1[A]): M1[Option[A]] =
		monadM1.bind(fa)(a => unit(a))
	override def unit[A](a: A): M1[Option[A]] = 
		monadM1.unit(Some(a))
}		
\end{lstlisting}		
	We can instantiate it on list, given  implicit ListMonad, in  this way:
\begin{lstlisting}[language=scala]
implicit object ListOptionT extends OptionT[List] {
	override implicit val monadM1: Monad[List] = implicitly
}
\end{lstlisting}
\end{frame}

\begin{frame}[fragile]{Transformer - Implementation (3)}	
	Through extension method we could also use transformer function as method in transformer:
\begin{lstlisting}[language=scala]
implicit class ToTransformer1[M1[_], M2[_], A, B](a: M1[M2[A]])(implicit transformer: Transformer[M1, M2]) {
	lazy val applyUnitT: A => M1[M2[A]] = transformer.unit
	def applyMapT(f: A => B): M1[M2[B]] = 
		transformer.map(a)(f)	
	def applyBindT(f: A => M1[M2[B]]): M1[M2[B]] = 
		transformer.bind(a)(f)
}
implicit class ToTransformer2[M1[_], M2[_], A, B](fa: M1[A])(implicit transformer: Transformer[M1, M2]) {
	lazy val applyLiftT: M1[M2[A]] = transformer.lift(fa)
}
implicit class ToTransformer3[M1[_], M2[_], A, B](fa: M1[M2[M1[M2[A]]]])(implicit transformer: Transformer[M1, M2]) {
	lazy val applyJoinT: M1[M2[A]] = transformer.join(fa)
}
\end{lstlisting}	
\end{frame}

\begin{frame}[fragile]{Transformer Laws}
	Transformer laws are expressed in scala in this way:
\begin{lstlisting}[language=scala]
def law1(a: A): Boolean = 
	transformer.monadM1.unit(a).applyLiftT == transformer.unit(a)
def law2(m: M1[A])(f: A => M1[A]): Boolean =
	transformer.lift(transformer.monadM1.bind(m)(f)) == transformer.lift(m).applyBindT(transformer.lift[A] _ compose f)
def leftIdentity(a: A)(f: A => M1[M2[A]]): Boolean = 
	transformer.unit(a).applyBindT(f) == f(a)
def rightIdentity(t: M1[M2[A]]): Boolean = 
	t.applyBindT(t.applyUnitT) == t
def associativity(t: M1[M2[A]])(f: A => M1[M2[A]], g: A => M1[M2[A]]): Boolean =
	t.applyBindT(f).applyBindT(g) == t.applyBindT((x: A) => f(x).applyBindT(g))
\end{lstlisting}	
	We could test these laws through PBT ScalaCheck.
\end{frame}